Extraction.v
@@ -1,8 +1,18 @@
-Require Import List Metatheory ML_SP_Domain.
+(***************************************************************************
+* Code extraction for structural polymorphism                              *
+* Jacques Garrigue, October 2007 - Jun 2009                                *
+***************************************************************************)
+
+Set Implicit Arguments.
+
+Require Import List Arith Metatheory ML_SP_Domain.
 Import Infer2.
 Import Sound3.
-Import Infer.Rename.Unify.MyEval.Sound.Infra.
+Import Infer.Rename.Unify.MyEval.
+Import Sound.Infra.
 Import Defs.
+Import Rename2.MyEval2.Sound2.JudgInfra.
+Import Judge.
 
 Definition t :=
   trm_app
@@ -12,7 +22,161 @@ Definition t :=
 (* This doesn't seem to work inside Coq (some things don't get evaluated) *)
 (* Eval compute in typinf' t. *)
 
-Definition eval' fenv t h := eval fenv h nil nil t nil.
+Definition decidable (A : Set) (P : A -> Prop) :=
+  forall x, sumbool (P x) (~P x).
+
+Definition ok_dec : decidable (@ok sch).
+  intro E; induction E.
+    left. apply ok_empty.
+  destruct IHE.
+    destruct a.
+    case_eq (get v E); intros.
+      right.
+      intro.
+      replace ((v,s)::E) with (E & v ~ s) in H0 by simpl*.
+      inversions H0.
+      elim (H5 (binds_dom H)).
+    left.
+    apply (@ok_push _ E v s o).
+    apply (get_none_notin  _ H).
+  right.
+  destruct a.
+  change (~ok (E & v ~ s)).
+  intro.
+  elim n.
+  inversion* H.
+Defined.
+
+Inductive type_n (n:nat) : typ -> Prop :=
+  | typn_bvar : forall m, m < n -> type_n n (typ_bvar m)
+  | typn_fvar : forall x, type_n n (typ_fvar x)
+  | typn_arrow : forall T1 T2,
+      type_n n T1 -> type_n n T2 -> type_n n (typ_arrow T1 T2).
+Hint Constructors type_n.
+
+Definition type_n_dec : forall n , decidable (type_n n).
+  introv T; induction T.
+    destruct (le_lt_dec n n0).
+      right. intro. inversions H. omega.
+    left*.
+   left*.
+  destruct IHT1.
+    destruct IHT2.
+      left*.
+    right; intro. inversions* H.
+  right; intro. inversions* H.
+Defined.
+
+Lemma type_n_typ_body : forall n T Xs,
+  n = length Xs -> 
+  (type_n n T <-> type (typ_open_vars T Xs)).
+Proof.
+  unfold typ_open_vars.
+  intros; split.
+    induction 1; simpl*.
+    destruct (types_typ_fvars Xs).
+    apply* (list_forall_out H2).
+    apply* nth_In.
+    rewrite <- H1; rewrite* <- H.
+  induction T; simpl; intros.
+      destruct* (le_lt_dec n n0).
+      rewrite H in l.
+      unfold typ_fvars in H0.
+      rewrite <- (map_length typ_fvar) in l.
+      rewrite (nth_overflow _ _ l) in H0. inversion H0.
+    auto.
+  inversions* H0.
+Qed.
+
+Definition list_forall_dec : forall (A:Set) (P:A->Prop),
+  decidable P -> decidable (list_forall P).
+  introv HP l; induction l.
+    left*.
+  destruct (HP a).
+    destruct* IHl.
+    right; intro. inversion* H.
+  right; intro. inversion* H.
+Defined.
+  
+Definition scheme_dec : decidable scheme.
+  intros [T Ks].
+  unfold scheme, typ_body; simpl.
+  set (n := length Ks). clearbody n.
+  destruct (type_n_dec n T).
+    puts (list_forall_dec (type_n_dec n)).
+    unfold All_kind_types.
+    puts (list_forall_dec (fun k => H (kind_types k))).
+    destruct (H0 Ks).
+      left; intuition. apply* (proj1 (type_n_typ_body T _ H1)).
+      apply* list_forall_imp; intros. simpl in H2.
+      apply* list_forall_imp; intros.
+      apply* (proj1 (type_n_typ_body x0 _ H1)).
+    right; intro.
+    elim n0; clear -H1.
+    destruct (var_freshes {} n).
+    destruct* (H1 x); clear H1.
+    apply* list_forall_imp; intros. simpl in H1.
+    refine (list_forall_imp _ _ H1); intros.
+    refine (proj2 (type_n_typ_body x1 _ _) H2); auto*.
+  right; intro.
+  elim n0; clear -H.
+  destruct (var_freshes {} n).
+  destruct* (H x); clear H.
+  refine (proj2 (type_n_typ_body T _ _) H0); auto*.
+Defined.
+
+Definition env_prop_dec : forall (A:Set) (P:A->Prop),
+  decidable P -> decidable (env_prop P).
+  introv HP E; induction E.
+    left; intro; intros. elim H.
+  destruct a.
+  destruct* (HP a).
+  destruct IHE.
+    left; intro; simpl; intros.
+    destruct* H.
+    inversions* H.
+  right; intro. elim n.
+  intro; auto*.
+Defined.
+
+Lemma env_weaker_refl : forall E, Rename2.env_weaker E E.
+Proof.
+  introv x; intros.
+  exists (@nil kind).
+  rewrite* <- app_nil_end.
+Qed.
+
+Definition typinf1 : forall E t,
+  sum (sig (fun p:kenv*typ => let (K,T) := p in K; E |Gc|= t ~: T))
+    (sumbool (env_fv E <> {}) (forall K T, ~ K;E |Gc|= t ~: T)).
+  intros.
+  case_eq (S.is_empty (env_fv E)); intros.
+    assert (Hempty: env_fv E = {}).
+      puts (S.is_empty_2 H).
+      apply eq_ext; split*. intro Ha; elim (H0 _ Ha).
+    clear H; destruct (ok_dec E).
+      destruct (env_prop_dec scheme_dec E).
+        case_eq (typinf' E t0); intros.
+          destruct p.
+          left.
+          exists (e0,t1).
+          apply* typinf_sound'. split*.
+        right; right; introv Typ.
+        destruct* (Rename2.typing_remove_gc Typ {} (@env_weaker_refl E))
+          as [K' [HK' Typ']].
+        destruct* (typinf_principal' Hempty Typ') as [K0 [T' [TI]]].
+        rewrite H in TI; discriminate.
+      right; right; introv Typ.
+      destruct* (proj42 (typing_regular Typ)).
+    right; right; introv Typ.
+    destruct* (proj42 (typing_regular Typ)).
+  right; left.
+  intro. rewrite H0 in H.
+  puts (S.is_empty_1 (S.empty_1)).
+  rewrite H1 in H; discriminate.
+Defined.
+
+Definition eval1 fenv t h := eval fenv h nil nil t nil.
 
 (* Export and try to do this in ocaml *)
-Extraction "typinf" typinf' eval'.
+Extraction "typinf" typinf1 eval1.
